src/dvspec/dafny/att_spec_proofs/proof_test.dfy
@@ -1,0 +1,31 @@
+include "../commons.dfy"
+include "../specification/dvc_spec.dfy"
+include "../specification/consensus.dfy"
+include "../specification/network.dfy"
+include "../specification/dvn.dfy"
+include "../att_spec_proofs/inv.dfy"
+include "../att_spec_proofs/assump.dfy"
+include "../att_spec_proofs/core_proofs.dfy"
+include "../att_spec_proofs/ci_ind_inv.dfy"
+include "../att_spec_proofs/dvc_ind_inv.dfy"
+include "../att_spec_proofs/dvn_ind_inv.dfy"
+
+module Proof_Test
+{
+    import opened Types 
+    import opened CommonFunctions
+    import opened ConsensusSpec
+    import opened NetworkSpec
+    import opened DVCNode_Spec
+    import opened DV
+    import opened Att_Inv_With_Empty_Initial_Attestation_Slashing_DB
+    import opened Att_Ind_Inv_With_Empty_Initial_Attestation_Slashing_DB
+    import opened Helper_Sets_Lemmas
+
+    lemma inv53(dvn: DVState, s: Slot)
+    ensures && var ci := dvn.consensus_on_attestation_data[s];
+            // && quorum(|ci.all_nodes|) <= |ci.honest_nodes_status|
+            && dvn.all_nodes == ci.all_nodes
+            && dvn.honest_nodes_states.Keys == ci.honest_nodes_status.Keys
+    {}
+}
